deps/poulet4/lib/P4cub/Semantics/Dynamic/BigStep/BigStep.v
@@ -1,8 +1,7 @@
-Set Warnings "-custom-entry-overridden".
 Require Export Poulet4.P4cub.Semantics.Climate.
 From Poulet4.P4cub.Semantics.Dynamic Require Export
      BigStep.Value.Value BigStep.ExprUtil
-     InstUtil BigStep.Semantics
+     BigStep.InstUtil BigStep.Semantics
      BigStep.IndPrincip BigStep.Determinism
      BigStep.TypeSoundness BigStep.Typing
      BigStep.Properties.
